Cedille/Lemma/BetaConv.lean
@@ -1,0 +1,96 @@
+
+import Cedille.Def
+import Cedille.Lemma.Erasure
+import Cedille.Lemma.Red
+import Cedille.Lemma.Confluence
+
+namespace Cedille.BetaConv
+
+  lemma refl : A =β= A := by {
+    apply BetaConv.conv RedStar.refl RedStar.refl
+  }
+
+  lemma symm : A =β= B -> B =β= A := by {
+    intros e; cases e; case _ t r1 r2 =>
+    apply BetaConv.conv r2 r1
+  }
+
+  lemma trans : A =β= B -> B =β= C -> A =β= C := by {
+    intro e1 e2
+    cases e1; case _ t1 r1 r2 =>
+    cases e2; case _ t2 w1 w2 =>
+    have r := confluence r2 w1
+    casesm* ∃ _, _, _ ∧ _; case _ Z q1 q2 =>
+    have r1' := RedStar.trans r1 q1
+    have r2' := RedStar.trans w2 q2
+    apply BetaConv.conv r1' r2'
+  }
+
+  lemma bind (x : Name) :
+    A =β= A' ->
+    x ∉ fv B ++ fv B' ->
+    {_|-> x}B =β= {_|-> x}B' ->
+    Syntax.bind k A B =β= Syntax.bind k A' B'
+  := by {
+    intro s1 xn s2
+    simp at *
+    replace xn := demorgan xn
+    cases xn; case _ xn1 xn2 =>
+    cases s1; case _ Az a1 a2 =>
+    cases s2; case _ Bz b1 b2 =>
+    apply BetaConv.conv _ _; exact Syntax.bind k Az ({_<-| x}Bz)
+    apply red_bind x a1 _ _
+    simp; intro h
+    cases h
+    case _ z => apply xn1 z
+    case _ z => apply var_not_in_close z
+    simp [*]
+    apply red_bind x a2 _ _
+    simp; intro h
+    cases h
+    case _ z => apply xn2 z
+    case _ z => apply var_not_in_close z
+    simp [*]
+  }
+
+  lemma bind1 :
+    A =β= A' ->
+    Syntax.bind k A B =β= Syntax.bind k A' B
+  := by sorry
+
+  lemma ctor :
+    A =β= A' ->
+    B =β= B' ->
+    C =β= C' ->
+    Syntax.ctor k A B C =β= Syntax.ctor k A' B' C'
+  := by {
+    intro c1 c2 c3
+    cases c1; case _ Az a1 a2 =>
+    cases c2; case _ Bz b1 b2 =>
+    cases c3; case _ Cz c1 c2 =>
+    apply BetaConv.conv _ _; exact Syntax.ctor k Az Bz Cz
+    apply red_ctor a1 b1 c1
+    apply red_ctor a2 b2 c2
+  }
+
+  lemma red_f : A =β= B -> A -β>* A' -> A' =β= B := by {
+    intro cv step
+    have cv2 : A' =β= A := BetaConv.symm (BetaConv.conv step RedStar.refl)
+    apply BetaConv.trans cv2 cv
+  }
+
+  lemma open_if (x : Name) : t =β= t' -> {_|-> x}t =β= {_|-> x}t' := by {
+    intro h
+    cases h; case _ z r1 r2 =>
+    sorry
+  }
+
+  -- lemma bind' {S : FvSet!} :
+  --   A =β= A' ->
+  --   ((x : Name) -> x ∉ S -> {_|-> x}B =β= {_|-> x}B') ->
+  --   Syntax.bind k A B =β= Syntax.bind k A' B'
+  -- := by {
+  --   sorry
+  -- }
+
+end Cedille.BetaConv
