Cedille/Lemma/Conv.lean
@@ -2,82 +2,9 @@
 import Cedille.Def
 import Cedille.Lemma.Erasure
 import Cedille.Lemma.Red
+import Cedille.Lemma.BetaConv
 import Cedille.Lemma.RedErasure
 import Cedille.Lemma.Confluence
-
-namespace Cedille.BetaConv
-
-  lemma refl : A =β= A := by {
-    apply BetaConv.conv RedStar.refl RedStar.refl
-  }
-
-  lemma symm : A =β= B -> B =β= A := by {
-    intros e; cases e; case _ t r1 r2 =>
-    apply BetaConv.conv r2 r1
-  }
-
-  lemma trans : A =β= B -> B =β= C -> A =β= C := by {
-    intro e1 e2
-    cases e1; case _ t1 r1 r2 =>
-    cases e2; case _ t2 w1 w2 =>
-    have r := confluence r2 w1
-    casesm* ∃ _, _, _ ∧ _; case _ Z q1 q2 =>
-    have r1' := RedStar.trans r1 q1
-    have r2' := RedStar.trans w2 q2
-    apply BetaConv.conv r1' r2'
-  }
-
-    lemma bind (x : Name) :
-    A =β= A' ->
-    x ∉ fv B ++ fv B' ->
-    {_|-> x}B =β= {_|-> x}B' ->
-    Syntax.bind k A B =β= Syntax.bind k A' B'
-  := by {
-    intro s1 xn s2
-    simp at *
-    replace xn := demorgan xn
-    cases xn; case _ xn1 xn2 =>
-    cases s1; case _ Az a1 a2 =>
-    cases s2; case _ Bz b1 b2 =>
-    apply BetaConv.conv _ _; exact Syntax.bind k Az ({_<-| x}Bz)
-    apply red_bind x a1 _ _
-    simp; intro h
-    cases h
-    case _ z => apply xn1 z
-    case _ z => apply var_not_in_close z
-    simp [*]
-    apply red_bind x a2 _ _
-    simp; intro h
-    cases h
-    case _ z => apply xn2 z
-    case _ z => apply var_not_in_close z
-    simp [*]
-  }
-
-  lemma ctor :
-    A =β= A' ->
-    B =β= B' ->
-    C =β= C' ->
-    Syntax.ctor k A B C =β= Syntax.ctor k A' B' C'
-  := by {
-    intro c1 c2 c3
-    cases c1; case _ Az a1 a2 =>
-    cases c2; case _ Bz b1 b2 =>
-    cases c3; case _ Cz c1 c2 =>
-    apply BetaConv.conv _ _; exact Syntax.ctor k Az Bz Cz
-    apply red_ctor a1 b1 c1
-    apply red_ctor a2 b2 c2
-  }
-
-  -- lemma bind' {S : FvSet!} :
-  --   A =β= A' ->
-  --   ((x : Name) -> x ∉ S -> {_|-> x}B =β= {_|-> x}B') ->
-  --   Syntax.bind k A B =β= Syntax.bind k A' B'
-  -- := by {
-  --   sorry
-  -- }
-
-end Cedille.BetaConv
 
 namespace Cedille.Conv
 
@@ -109,42 +36,44 @@ namespace Cedille.Conv
   }
 
   lemma red_f :
-    Sane a ->
+    PseObj a ->
     a === b ->
     a -β>* a' ->
     a' === b
   := by {
-    intro h cv step
-    cases cv; case _ u v r1 e r2 =>
-    have lem1 := confluence step r1
-    casesm* ∃ _, _, _ ∧ _; case _ z r3 r4 =>
-    have lem2 := preservation_of_sanity h r1
-    replace e := erase_red_f lem2 e r4
-    constructor; exact r3; exact r2; exact e
+    sorry
+    -- intro h cv step
+    -- cases cv; case _ u v r1 e r2 =>
+    -- have lem1 := confluence step r1
+    -- casesm* ∃ _, _, _ ∧ _; case _ z r3 r4 =>
+    -- have lem2 := preservation_of_sanity h r1
+    -- replace e := erase_red_f lem2 e r4
+    -- constructor; exact r3; exact r2; exact e
   }
 
   lemma trans :
-    Sane B ->
+    PseObj B ->
     A === B ->
     B === C ->
     A === C
   := by {
-    intro h c1 c2
-    cases c1; case _ u1 u2 r1 e1 r2 =>
-    cases c2; case _ v1 v2 r3 e2 r4 =>
-    have lem := confluence r2 r3
-    casesm* ∃ _, _, _ ∧ _; case _ B' rr1 rr2 =>
-    constructor; exact r1; exact r4
-    intro x
-    have h2 : Sane u2 := preservation_of_sanity h r2
-    have h3 : Sane v1 := preservation_of_sanity h r3
-    replace e1 := erase_red_f h2 (λ x => BetaConv.symm (e1 x)) rr1
-    replace e2 := erase_red_f h3 e2 rr2
-    have lem := BetaConv.trans (BetaConv.symm (e1 x)) (e2 x)
-    exact lem
+    sorry
+    -- intro h c1 c2
+    -- cases c1; case _ u1 u2 r1 e1 r2 =>
+    -- cases c2; case _ v1 v2 r3 e2 r4 =>
+    -- have lem := confluence r2 r3
+    -- casesm* ∃ _, _, _ ∧ _; case _ B' rr1 rr2 =>
+    -- constructor; exact r1; exact r4
+    -- intro x
+    -- have h2 : PseObj u2 := preservation_of_sanity h r2
+    -- have h3 : PseObj v1 := preservation_of_sanity h r3
+    -- replace e1 := erase_red_f h2 (λ x => BetaConv.symm (e1 x)) rr1
+    -- replace e2 := erase_red_f h3 e2 rr2
+    -- have lem := BetaConv.trans (BetaConv.symm (e1 x)) (e2 x)
+    -- exact lem
   }
 
-  lemma to_beta (S : FvSet!) : Sane a -> Sane b -> a === b -> (∀ x, erase x a =β= erase x b)
+  lemma to_beta (S : FvSet!) : PseObj a -> PseObj b -> a === b -> (∀ x, erase x a =β= erase x b)
   := by {
     intro h1 h2 cv
     cases cv; case _ a' b' r1 e r2 =>
