Cedille/Lemma/PseObj.lean
@@ -1,0 +1,13 @@
+
+import Common
+import Cedille.Def
+import Cedille.Lemma.Refold
+import Cedille.Lemma.Inversion
+import Cedille.Lemma.Syntax
+
+namespace Cedille
+
+  -- Not yet used
+  lemma pseobj_open : PseObj ({_|-> x}t) -> PseObj ({_|-> y}t) := by sorry
+
+end Cedille
