Cedille/Lemma/Rule.lean
@@ -40,77 +40,77 @@ namespace Cedille
     intro j; apply ConInfer.infer j RedStar.refl
   }
 
-  lemma infer_implies_sane : Γ ⊢ t : A -> Sane t := λ j => @Infer.rec
-    (λ Γ t A _ => Sane t)
-    (λ Γ t A _ => Sane t)
-    (λ Γ t A _ => Sane t)
-    (λ Γ _ => True)
-    (by intros; constructor)
-    (by intros; constructor)
-    (by {
-      intro Γ A m K B S j1 j2 ih1 ih2
-      simp at *
-      constructor; exact ih1; exact ih2
-    })
-    (by {
-      intros Γ A m K t B S j1 j2 j3 ih1 ih2
-      simp at *
-      constructor; exact ih1; exact ih2; exact j3
-    })
-    (by {
-      intro Γ f m A B a S j1 j2 ih1 ih2
-      constructor; exact ih1; exact ih2
-    })
-    (by {
-      intro Γ A B S j1 j2 ih1 ih2
-      simp at *
-      constructor; exact ih1; exact ih2
-    })
-    (by {
-      intro Γ T A B t s S j1 j2 j3 j4 ih1 ih2 ih3
-      constructor; exact ih1; exact ih2; exact ih3; exact j4
-    })
-    (by {
-      intro Γ t A B j ih
-      constructor; exact ih
-    })
-    (by {
-      intro Γ t A B j ih
-      constructor; exact ih
-    })
-    (by {
-      intro Γ A a b j1 j2 j3 ih1 ih2 ih3
-      constructor; exact ih1; exact ih2; exact ih3
-    })
-    (by {
-      intro Γ t A j ih
-      constructor; exact ih
-    })
-    (by {
-      intro Γ A P x y r w j1 j2 j3 j4 j5 j6 ih1 ih2 ih3 ih4 ih5 ih6
-      constructor; exact ih1; exact ih2; exact ih3
-      exact ih4; exact ih5; exact ih6
-    })
-    (by {
-      intro Γ e T a b A B j1 j2 j3 j4 ih1 ih2 ih3
-      constructor; exact ih1
-    })
-    (by {
-      intro Γ f A B a e j1 j2 j3 j4 ih1 ih2 ih3
-      constructor; exact ih2; exact ih1; exact ih3
-    })
-    (by {
-      intro Γ e j ih
-      constructor; exact ih
-    })
-    (by intros; simp [*])
-    (by intros; simp [*])
-    (by simp)
-    (by simp)
-    Γ
-    t
-    A
-    j
+  lemma infer_implies_pseobj : Γ ⊢ t : A -> PseObj t := by sorry --λ j => @Infer.rec
+    -- (λ Γ t A _ => PseObj t)
+    -- (λ Γ t A _ => PseObj t)
+    -- (λ Γ t A _ => PseObj t)
+    -- (λ Γ _ => True)
+    -- (by intros; constructor)
+    -- (by intros; constructor)
+    -- (by {
+    --   intro Γ A m K B S j1 j2 ih1 ih2
+    --   simp at *
+    --   constructor; exact ih1; exact ih2
+    -- })
+    -- (by {
+    --   intros Γ A m K t B S j1 j2 j3 ih1 ih2
+    --   simp at *
+    --   constructor; exact ih1; exact ih2; exact j3
+    -- })
+    -- (by {
+    --   intro Γ f m A B a S j1 j2 ih1 ih2
+    --   constructor; exact ih1; exact ih2
+    -- })
+    -- (by {
+    --   intro Γ A B S j1 j2 ih1 ih2
+    --   simp at *
+    --   constructor; exact ih1; exact ih2
+    -- })
+    -- (by {
+    --   intro Γ T A B t s S j1 j2 j3 j4 ih1 ih2 ih3
+    --   constructor; exact ih1; exact ih2; exact ih3; exact j4
+    -- })
+    -- (by {
+    --   intro Γ t A B j ih
+    --   constructor; exact ih
+    -- })
+    -- (by {
+    --   intro Γ t A B j ih
+    --   constructor; exact ih
+    -- })
+    -- (by {
+    --   intro Γ A a b j1 j2 j3 ih1 ih2 ih3
+    --   constructor; exact ih1; exact ih2; exact ih3
+    -- })
+    -- (by {
+    --   intro Γ t A j ih
+    --   constructor; exact ih
+    -- })
+    -- (by {
+    --   intro Γ A P x y r w j1 j2 j3 j4 j5 j6 ih1 ih2 ih3 ih4 ih5 ih6
+    --   constructor; exact ih1; exact ih2; exact ih3
+    --   exact ih4; exact ih5; exact ih6
+    -- })
+    -- (by {
+    --   intro Γ e T a b A B j1 j2 j3 j4 ih1 ih2 ih3
+    --   constructor; exact ih1
+    -- })
+    -- (by {
+    --   intro Γ f A B a e j1 j2 j3 j4 ih1 ih2 ih3
+    --   constructor; exact ih2; exact ih1; exact ih3
+    -- })
+    -- (by {
+    --   intro Γ e j ih
+    --   constructor; exact ih
+    -- })
+    -- (by intros; simp [*])
+    -- (by intros; simp [*])
+    -- (by simp)
+    -- (by simp)
+    -- Γ
+    -- t
+    -- A
+    -- j
 
   lemma chck_type_red : Γ ⊢ t =: A -> A -β>* B -> Γ ⊢ t =: B := by {
     intro j step
