Cedille/Lemma/Substitution.lean
@@ -7,14 +7,98 @@ import Cedille.Lemma.Syntax
 
 namespace Cedille
 
+  lemma subst_erase {n} (t1 : Term n) (t2 : Term (n + 1))
+    : erase x ([_:= t1]t2) = [_:= erase x t1]erase x t2
+  := @Nat.rec
+    (λ s => ∀ {n} {t1:Term n} {t2: Term (n + 1)},
+      size t2 ≤ s ->
+      erase x ([_:= t1]t2) = [_:= erase x t1]erase x t2)
+    sorry
+    (by {
+      intro s ih n t1 t2 sh
+      sorry
+    })
+    (size t2)
+    n
+    t1
+    t2
+    (by simp)
+
+
+  -- lemma subst_erase (S : FvSet!) {t1 : Term 0} {t2 : Term 1}
+  --   : (∀ x ∉ S, PseObj ({_|-> x}t2)) ->
+  --     erase x ([_:= t1]t2) = [_:= erase x t1]erase x t2
+  -- := @Nat.rec
+  --   (λ s => ∀ {n:Nat} {t1:Term n} {t2:Term (n + 1)},
+  --     size t2 ≤ s ->
+  --     (∀ x ∉ S, x ∉ (fv ∘ erase x) ({_|-> x}t)) ->
+  --     erase x ([_:= t1]t2) = [_:= erase x t1]erase x t2)
+  --   sorry
+  --   (by {
+  --     intro s ih n' t1 t2 sh h
+  --     cases t2 <;> simp at sh
+  --     case bound j => apply @ih _ t1 (bound j) (by simp) h
+  --     case free x => apply @ih _ t1 (free x) (by simp) h
+  --     case const k => apply @ih _ t1 (const k) (by simp) h
+  --     case bind k u1 u2 => {
+  --       have sh1 : size u1 ≤ s := by linarith
+  --       have sh2 : size u2 ≤ s := by linarith
+  --       cases k <;> simp at *
+  --       case lam md => {
+  --         cases md
+  --         case free => sorry
+  --         case type => sorry
+  --         case erased => {
+
+  --           sorry
+  --         }
+  --       }
+  --       case pi md => sorry
+  --       case inter => sorry
+  --     }
+  --     case ctor k u1 u2 u3 => {
+  --       have sh1 : size u1 ≤ s := by linarith
+  --       have sh2 : size u2 ≤ s := by linarith
+  --       have sh3 : size u3 ≤ s := by linarith
+  --       cases k <;> simp at *
+  --       case app md => {
+  --         cases md <;> simp at *
+  --         case free => rw [ih sh1, ih sh2]
+  --         case type => rw [ih sh1, ih sh2]
+  --         case erased => apply ih sh1
+  --       }
+  --       case pair => apply ih sh1
+  --       case fst => apply ih sh1
+  --       case snd => apply ih sh1
+  --       case eq => rw [ih sh1, ih sh2, ih sh3]
+  --       case refl => {
+  --         unfold HasHSubst.hsubst; unfold Syntax.instHasHSubstSyntax; simp
+  --         unfold Syntax.hsubst; unfold bound; simp
+  --         split
+  --         case _ h => exfalso; linarith
+  --         case _ => simp
+  --       }
+  --       case eqind => rw [ih sh3]
+  --       case jω => rw [ih sh1, ih sh2]
+  --       case promote => rw [ih sh1]
+  --       case delta => rw [ih sh1]
+  --       case phi => rw [ih sh1]
+  --     }
+  --   })
+  --   (size t2)
+  --   t1
+  --   t2
+  --   (by simp)
+
+
   lemma subst_hsubst_commute {t1 t2 : Term n} {t3 : Term (n + 1)} :
     [x := t1][_:= t2]t3 = [_:= [x := t1]t2][x := t1ʷ]t3
   := by sorry
 
-  lemma sanity_subst {S : FvSet!} :
-    Sane a ->
-    (∀ x, x ∉ S -> Sane ({_|-> x}f)) ->
-    Sane ([_:= a]f)
-  := by sorry
+  -- lemma subst_pseobj {S : FvSet!} :
+  --   PseObj a ->
+  --   (∀ x, x ∉ S -> PseObj ({_|-> x}f)) ->
+  --   PseObj ([_:= a]f)
+  -- := by sorry
 
 end Cedille
